Valaig/Aig/Semantics.lean
@@ -15,131 +15,395 @@ An timeframe (step) index of the model.
 -/
 abbrev Frame := Nat
 
-variable {var : Var} {lit : Lit} {frame : Frame}
-variable {valid : var.validIn aig} {litValid : lit.validIn aig} {wf : aig.WellFormed}
-
-mutual
-
+/--
+Combinational (uninitialised) denotation of literals.
+-/
 @[expose]
-def denoteCombVar (aig : Aig) (var : Var) (assign : LeafIdx -> Bool)
-      (wf : aig.WellFormed := by grind) : Bool :=
-    match _ : aig[var]? with
+def denoteC (aig : Aig) (lit : Lit) (assign : LeafIdx -> Frame -> Bool) (frame : Frame := 0)
+    (wf : aig.WellFormed := by grind) :=
+  lit.inverted ^^
+    match _ : aig[lit.var]? with
     | none
     | some .false           => false
-    | some (.input idx)
-    | some (.latch idx)     => assign idx
-    | some (.and rhs0 rhs1) => aig.denoteComb rhs0 assign && aig.denoteComb rhs1 assign
-  termination_by (var, 0)
-  decreasing_by all_goals grind
+    | some (.input idx)     => assign idx frame
+    | some (.latch idx)     =>
+      match frame with
+      | 0                   => assign idx 0
+      | n + 1               => aig.denoteC (idx.getNext aig) assign n
+    | some (.and rhs0 rhs1) => aig.denoteC rhs0 assign frame && aig.denoteC rhs1 assign frame
+termination_by (frame, lit.var)
+decreasing_by all_goals grind
 
-def denoteComb (aig : Aig) (lit : Lit) (assign : LeafIdx -> Bool)
-      (wf : aig.WellFormed := by grind) : Bool :=
-    lit.inverted ^^ aig.denoteCombVar lit.var assign wf
-  termination_by (lit.var, 1)
+@[expose]
+def denoteC.assignNext (aig : Aig) (frame : Frame) (assign : LeafIdx -> Frame -> Bool)
+    (wf : aig.WellFormed := by grind) : LeafIdx -> Frame -> Bool :=
+  fun idx _ =>
+    match _ : decide (idx.validIn aig), _ : idx, _ : frame with
+    | true, .latch idx, n + 1 => aig.denoteC (idx.getNext aig) assign n
+    |    _,          _,     _ => assign idx frame
 
-end -- mutual
+/--
+Combinational (uninitialised) denotation of variables.
+-/
+@[expose]
+def denoteCV (aig : Aig) (var : Var) (assign : LeafIdx -> Frame -> Bool) (frame : Frame := 0)
+    (wf : aig.WellFormed := by grind) :=
+  aig.denoteC var.toLit assign frame wf
+
+/--
+Sequential (initialised) denotation of literals.
+-/
+@[expose]
+def denoteS (aig : Aig) (lit : Lit) (assign : LeafIdx -> Frame -> Bool) (frame : Frame := 0)
+    (wf : aig.WellFormed := by grind) :=
+  lit.inverted ^^
+    match _ : aig[lit.var]? with
+    | none
+    | some .false           => false
+    | some (.input idx)     => assign idx frame
+    | some (.latch idx)     =>
+      match frame with
+      | 0                   =>
+        match _ : idx.getReset aig with
+        | none              => assign idx 0
+        | some reset        => aig.denoteS reset assign 0
+      | n + 1               => aig.denoteS (idx.getNext aig) assign n
+    | some (.and rhs0 rhs1) => aig.denoteS rhs0 assign frame && aig.denoteS rhs1 assign frame
+termination_by (frame, lit.var)
+decreasing_by all_goals grind
+
+@[expose]
+def denoteS.assignNext (aig : Aig) (frame : Frame) (assign : LeafIdx -> Frame -> Bool)
+    (wf : aig.WellFormed := by grind) : LeafIdx -> Frame -> Bool :=
+  fun idx _ =>
+    match _ : decide (idx.validIn aig), _ : idx, _ : frame with
+    | true, .latch idx, 0     =>
+      match idx.getReset aig with
+      | none                  => assign idx 0
+      | some reset            => aig.denoteS reset assign 0
+    | true, .latch idx, n + 1 => aig.denoteS (idx.getNext aig) assign n
+    |    _,          _,     _ => assign idx frame
+
+/--
+Sequential (initialised) denotation of variables.
+-/
+@[expose]
+def denoteSV (aig : Aig) (var : Var) (assign : LeafIdx -> Frame -> Bool) (frame : Frame := 0)
+    (wf : aig.WellFormed := by grind) :=
+  aig.denoteS var.toLit assign frame wf
+
+scoped syntax "⟦" term ", " term ", " term (", " term)? ("⟧c" <|> "⟧cv" <|> "⟧s" <|> "⟧sv") (num)? : term
+
+scoped macro_rules
+| `(⟦$aig, $lit,         $assign⟧c$frame)  => `(denoteC  $aig $lit $assign $frame)
+| `(⟦$aig, $var,         $assign⟧cv$frame) => `(denoteCV $aig $var $assign $frame)
+| `(⟦$aig, $lit,         $assign⟧s$frame)  => `(denoteS  $aig $lit $assign $frame)
+| `(⟦$aig, $var,         $assign⟧sv$frame) => `(denoteSV $aig $var $assign $frame)
+| `(⟦$aig, $lit, $frame, $assign⟧c)        => `(denoteC  $aig $lit $assign $frame)
+| `(⟦$aig, $var, $frame, $assign⟧cv)       => `(denoteCV $aig $var $assign $frame)
+| `(⟦$aig, $lit, $frame, $assign⟧s)        => `(denoteS  $aig $lit $assign $frame)
+| `(⟦$aig, $var, $frame, $assign⟧sv)       => `(denoteSV $aig $var $assign $frame)
+
+@[app_unexpander Aig.denoteC]
+meta def unexpandDenoteC : Lean.PrettyPrinter.Unexpander
+  | `($(_) $aig $lit $assign      0 $_) => `(⟦$aig, $lit, $assign⟧c0)
+  | `($(_) $aig $lit $assign      1 $_) => `(⟦$aig, $lit, $assign⟧c1)
+  | `($(_) $aig $lit $assign $frame $_) => `(⟦$aig, $lit, $frame, $assign⟧c)
+  | _ => throw ()
+
+@[app_unexpander Aig.denoteCV]
+meta def unexpandDenoteCV : Lean.PrettyPrinter.Unexpander
+  | `($(_) $aig $var $assign      0 $_) => `(⟦$aig, $var, $assign⟧cv0)
+  | `($(_) $aig $var $assign      1 $_) => `(⟦$aig, $var, $assign⟧cv1)
+  | `($(_) $aig $var $assign $frame $_) => `(⟦$aig, $var, $frame, $assign⟧cv)
+  | _ => throw ()
+
+@[app_unexpander Aig.denoteS]
+meta def unexpandDenoteS : Lean.PrettyPrinter.Unexpander
+  | `($(_) $aig $lit $assign      0 $_) => `(⟦$aig, $lit, $assign⟧s0)
+  | `($(_) $aig $lit $assign      1 $_) => `(⟦$aig, $lit, $assign⟧s1)
+  | `($(_) $aig $lit $assign $frame $_) => `(⟦$aig, $lit, $frame, $assign⟧s)
+  | _ => throw ()
+
+@[app_unexpander Aig.denoteSV]
+meta def unexpandDenoteSV : Lean.PrettyPrinter.Unexpander
+  | `($(_) $aig $var $assign      0 $_) => `(⟦$aig, $var, $assign⟧sv0)
+  | `($(_) $aig $var $assign      1 $_) => `(⟦$aig, $var, $assign⟧sv1)
+  | `($(_) $aig $var $assign $frame $_) => `(⟦$aig, $var, $frame, $assign⟧sv)
+  | _ => throw ()
+
+variable {wf : aig.WellFormed} {assign : LeafIdx -> Frame -> Bool} {frame : Frame} {lit : Lit} {var : Var}
 
 /-
-Semantics to elements in the aig for `denoteComb`
+Locally we provide extra syntax that automatically assumes it is working within aig/frame to
+keep definitions simpler to read.
 -/
-section denoteComb
-variable {assign : LeafIdx -> Bool}
+local syntax "⟦" term (", " term)? ("⟧c" <|> "⟧cv" <|> "⟧s" <|> "⟧sv") (num)? : term
+local macro_rules
+| `(⟦$lit⟧c)          => `(denoteC  aig $lit assign frame  wf)
+| `(⟦$lit⟧cv)         => `(denoteCV aig $lit assign frame  wf)
+| `(⟦$lit⟧s)          => `(denoteS  aig $lit assign frame  wf)
+| `(⟦$lit⟧sv)         => `(denoteSV aig $lit assign frame  wf)
+| `(⟦$lit⟧c$frame)    => `(denoteC  aig $lit assign $frame wf)
+| `(⟦$lit⟧cv$frame)   => `(denoteCV aig $lit assign $frame wf)
+| `(⟦$lit⟧s$frame)    => `(denoteS  aig $lit assign $frame wf)
+| `(⟦$lit⟧sv$frame)   => `(denoteSV aig $lit assign $frame wf)
+| `(⟦$lit, $frame⟧c)  => `(denoteC  aig $lit assign $frame wf)
+| `(⟦$lit, $frame⟧cv) => `(denoteCV aig $lit assign $frame wf)
+| `(⟦$lit, $frame⟧s)  => `(denoteS  aig $lit assign $frame wf)
+| `(⟦$lit, $frame⟧sv) => `(denoteSV aig $lit assign $frame wf)
 
-@[simp, grind =]
-theorem denoteComb_eq :
-    aig.denoteComb lit assign wf =
-    (lit.inverted ^^ aig.denoteCombVar lit.var assign wf) := by
-  unfold denoteComb
-  grind
-
-@[simp]
-theorem denoteCombVar_invalid (invalid : ¬var.validIn aig) :
-    aig.denoteCombVar var assign wf = false := by
-  unfold denoteCombVar
-  grind
-
-grind_pattern denoteCombVar_invalid => aig.denoteCombVar var assign wf, var.validIn aig
-
-@[simp, grind =]
-theorem denoteCombVar_constant :
-    aig.denoteCombVar .constant assign wf = false := by
-  unfold denoteCombVar
-  grind
-
-@[simp]
-theorem denoteCombVar_get_false (h : aig.get var valid = .false) :
-    aig.denoteCombVar var assign wf = false := by
-  grind
-
-grind_pattern denoteCombVar_get_false => aig.get var, Node.false, aig.denoteCombVar var assign wf
-
-@[simp]
-theorem denoteCombVar_get_input {idx : InputIdx} (h : aig.get var valid = .input idx) :
-    aig.denoteCombVar var assign wf = assign idx := by
-  unfold denoteCombVar
-  grind
-
-grind_pattern denoteCombVar_get_input => aig.get var, Node.input idx, aig.denoteCombVar var assign wf where
-  var =/= idx.getVar aig
-  idx =/= (_ : Aig).addInput.snd
-
-@[simp, grind =]
-theorem denoteCombVar_input_getVar {idx : InputIdx} (valid : idx.validIn aig) :
-    aig.denoteCombVar (idx.getVar aig valid) assign wf = assign idx := by
-  grind [get_input_getVar, denoteCombVar_get_input]
-
-@[simp]
-theorem denoteCombVar_get_latch {idx : LatchIdx} (h : aig.get var valid = .latch idx) :
-    aig.denoteCombVar var assign wf = assign idx := by
-  unfold denoteCombVar
-  grind
-
-grind_pattern denoteCombVar_get_latch => aig.get var, Node.latch idx, aig.denoteCombVar var assign wf where
-  var =/= idx.getVar aig
-  idx =/= ((_ : Aig).addLatch _ _).snd
-
-@[simp, grind =]
-theorem denoteCombVar_latch_getVar {idx : LatchIdx} (valid : idx.validIn aig) :
-    aig.denoteCombVar (idx.getVar aig valid) assign wf = assign idx := by
-  grind [get_latch_getVar, denoteCombVar_get_latch]
-
-@[simp]
-theorem denoteCombVar_get_and {rhs0 rhs1 : Lit} (h : aig.get var valid = .and rhs0 rhs1) :
-    aig.denoteCombVar var assign wf =
-      (aig.denoteComb rhs0 assign wf && aig.denoteComb rhs1 assign wf) := by
-  rw [denoteCombVar]
-  grind
-
-grind_pattern denoteCombVar_get_and => aig.get var, Node.and rhs0 rhs1, aig.denoteCombVar var assign wf
-
-theorem denoteCombVar_eq_of_le (assign assign' : LeafIdx -> Bool)
-    (h : {idx : LeafIdx} -> (valid : idx.validIn aig) -> idx.getVar aig valid ≤ var -> assign' idx = assign idx) :
-    aig.denoteCombVar var assign' wf = aig.denoteCombVar var assign wf := by
-  induction var using WellFounded.induction
+theorem denoteC_zero_eq_assign_zero :
+    ⟦lit⟧c0 = ⟦aig, lit, fun idx _ => assign idx 0⟧c0 := by
+  induction h : lit.var using WellFounded.induction generalizing lit
   exact WellFoundedRelation.wf
   next ih =>
     simp only [WellFoundedRelation.rel] at ih
-    unfold denoteCombVar
-    split <;> grind (ematch := 10)
+    unfold denoteC
+    unfold denoteC.assignNext at *
+    split <;> grind
+
+theorem denoteS_zero_eq_assign_zero :
+    ⟦lit⟧s0 =
+    ⟦aig, lit, fun idx _ => assign idx 0⟧s0 := by
+  induction h : lit.var using WellFounded.induction generalizing lit
+  exact WellFoundedRelation.wf
+  next ih =>
+    simp only [WellFoundedRelation.rel] at ih
+    unfold denoteS
+    unfold denoteS.assignNext at *
+    split <;> grind
+
+theorem denoteCV_zero_eq_assign_zero :
+    ⟦var⟧cv0 = ⟦aig, var, fun idx _ => assign idx 0⟧cv0 := by
+  grind [denoteCV, denoteC_zero_eq_assign_zero]
+
+theorem denoteSV_zero_eq_assign_zero :
+    ⟦var⟧sv0 = ⟦aig, var, fun idx _ => assign idx 0⟧sv0 := by
+  grind [denoteSV, denoteS_zero_eq_assign_zero]
+
+theorem denoteC_eq_denoteC_assignNext :
+    ⟦lit⟧c = ⟦aig, lit, denoteC.assignNext aig frame assign⟧c0 := by
+  induction h : lit.var using WellFounded.induction generalizing lit
+  exact WellFoundedRelation.wf
+  next ih =>
+    simp only [WellFoundedRelation.rel] at ih
+    unfold denoteC
+    unfold denoteC.assignNext at *
+    split <;> grind
+
+theorem denoteS_eq_denoteC_assignNext :
+    ⟦lit⟧s = ⟦aig, lit, denoteS.assignNext aig frame assign⟧c0 := by
+  induction h : lit.var using WellFounded.induction generalizing lit
+  exact WellFoundedRelation.wf
+  next ih =>
+    simp only [WellFoundedRelation.rel] at ih
+    unfold denoteS denoteC
+    unfold denoteS.assignNext at *
+    split <;> grind
+
+theorem denoteCV_eq_denoteCV_assignNext :
+    ⟦var⟧cv = ⟦aig, var, denoteC.assignNext aig frame assign⟧cv0 := by
+  grind [denoteCV, denoteC_eq_denoteC_assignNext]
+
+theorem denoteSV_eq_denoteCV_assignNext :
+    ⟦var⟧sv = ⟦aig, var, denoteS.assignNext aig frame assign⟧cv0 := by
+  rw [denoteSV, denoteS_eq_denoteC_assignNext, denoteCV]
+
+@[simp, grind =]
+theorem denoteC_assignNext_zero {idx : LeafIdx} {f : Frame} :
+    (denoteC.assignNext aig 0 assign wf) idx f = assign idx 0 := by
+  unfold denoteC.assignNext
+  split <;> grind
+
+@[local grind =] theorem denoteC_eq : ⟦lit⟧c = (lit.inverted ^^ ⟦lit.var⟧cv) := by grind [denoteC, denoteCV]
+@[local grind =] theorem denoteS_eq : ⟦lit⟧s = (lit.inverted ^^ ⟦lit.var⟧sv) := by grind [denoteS, denoteSV]
+grind_pattern denoteC_eq => ⟦aig, lit, frame, assign⟧c, lit.var
+grind_pattern denoteS_eq => ⟦aig, lit, frame, assign⟧s, lit.var
+
+theorem denoteCV_eq : ⟦var⟧cv = ⟦var.toLit⟧c := by grind [denoteCV]
+theorem denoteSV_eq : ⟦var⟧sv = ⟦var.toLit⟧s := by grind [denoteSV]
+
+@[simp] theorem denoteC_false : ⟦.false⟧c = .false := by grind [denoteC]
+@[simp] theorem denoteS_false : ⟦.false⟧s = .false := by grind [denoteS]
+@[simp] theorem denoteC_true : ⟦.true⟧c = .true := by grind [denoteC]
+@[simp] theorem denoteS_true : ⟦.true⟧s = .true := by grind [denoteS]
+@[simp] theorem denoteC_constant {value : Bool} : ⟦.constant value⟧c = value := by grind [denoteC]
+@[simp] theorem denoteS_constant {value : Bool} : ⟦.constant value⟧s = value := by grind [denoteS]
+@[simp, grind =] theorem denoteCV_constant : ⟦.constant⟧cv = .false := by grind [denoteCV_eq, denoteC]
+@[simp, grind =] theorem denoteSV_constant : ⟦.constant⟧sv = .false := by grind [denoteSV_eq, denoteS]
+
+@[simp] theorem denoteC_not_inverted  (h : ¬lit.inverted) : ⟦lit    ⟧c  =  ⟦lit.var⟧cv := by grind
+@[simp] theorem denoteS_not_inverted  (h : ¬lit.inverted) : ⟦lit    ⟧s  =  ⟦lit.var⟧sv := by grind
+@[simp] theorem denoteC_inverted      (h :  lit.inverted) : ⟦lit    ⟧c  = !⟦lit.var⟧cv := by grind
+@[simp] theorem denoteS_inverted      (h :  lit.inverted) : ⟦lit    ⟧s  = !⟦lit.var⟧sv := by grind
+@[simp] theorem denoteCV_not_inverted (h : ¬lit.inverted) : ⟦lit.var⟧cv =  ⟦lit    ⟧c := by grind
+@[simp] theorem denoteSV_not_inverted (h : ¬lit.inverted) : ⟦lit.var⟧sv =  ⟦lit    ⟧s := by grind
+@[simp] theorem denoteCV_inverted     (h :  lit.inverted) : ⟦lit.var⟧cv = !⟦lit    ⟧c := by grind
+@[simp] theorem denoteSV_inverted     (h :  lit.inverted) : ⟦lit.var⟧sv = !⟦lit    ⟧s := by grind
+
+@[simp] theorem denoteCV_var_eq : ⟦lit.var⟧cv = (lit.inverted ^^ ⟦lit⟧c) := by grind
+@[simp] theorem denoteSV_var_eq : ⟦lit.var⟧sv = (lit.inverted ^^ ⟦lit⟧s) := by grind
+grind_pattern denoteCV_var_eq => ⟦aig, lit.var, frame, assign⟧cv where lit =/= Lit.mk _ _
+grind_pattern denoteSV_var_eq => ⟦aig, lit.var, frame, assign⟧sv where lit =/= Lit.mk _ _
+
+@[simp, grind =] theorem denoteC_mk {var : Var} {invert : Bool} : ⟦.mk var invert⟧c = (invert ^^ ⟦var⟧cv) := by grind
+@[simp, grind =] theorem denoteS_mk {var : Var} {invert : Bool} : ⟦.mk var invert⟧s = (invert ^^ ⟦var⟧sv) := by grind
+
+@[simp] theorem denoteC_invalid  (invalid : ¬lit.validIn aig) : ⟦lit⟧c  = decide lit.inverted := by grind [denoteC]
+@[simp] theorem denoteS_invalid  (invalid : ¬lit.validIn aig) : ⟦lit⟧s  = decide lit.inverted := by grind [denoteS]
+@[simp] theorem denoteCV_invalid (invalid : ¬var.validIn aig) : ⟦var⟧cv = false               := by grind [denoteCV_eq, denoteC_invalid]
+@[simp] theorem denoteSV_invalid (invalid : ¬var.validIn aig) : ⟦var⟧sv = false               := by grind [denoteSV_eq, denoteS_invalid]
+grind_pattern denoteC_invalid  => ⟦aig, lit, frame, assign⟧c, lit.validIn aig
+grind_pattern denoteS_invalid  => ⟦aig, lit, frame, assign⟧s, lit.validIn aig
+grind_pattern denoteCV_invalid => ⟦aig, var, frame, assign⟧cv, var.validIn aig
+grind_pattern denoteSV_invalid => ⟦aig, var, frame, assign⟧sv, var.validIn aig
+
+section get
+variable {valid : var.validIn aig}
+
+@[simp] theorem denoteCV_get_false (h : aig.get var valid = .false) : ⟦var⟧cv = false := by grind [denoteCV_eq, denoteC]
+@[simp] theorem denoteSV_get_false (h : aig.get var valid = .false) : ⟦var⟧sv = false := by grind [denoteSV_eq, denoteS]
+grind_pattern denoteCV_get_false => aig.get var, Node.false, ⟦aig, var, frame, assign⟧cv
+grind_pattern denoteSV_get_false => aig.get var, Node.false, ⟦aig, var, frame, assign⟧sv
+
+@[simp] theorem denoteCV_get_input {idx : InputIdx} (h : aig.get var valid = .input idx) : ⟦var⟧cv = assign idx frame := by grind [denoteCV_eq, denoteC]
+@[simp] theorem denoteSV_get_input {idx : InputIdx} (h : aig.get var valid = .input idx) : ⟦var⟧sv = assign idx frame := by grind [denoteSV_eq, denoteS]
+grind_pattern denoteCV_get_input => aig.get var, Node.input idx, ⟦aig, var, frame, assign⟧cv where idx =/= (_ : Aig).addInput.snd
+grind_pattern denoteSV_get_input => aig.get var, Node.input idx, ⟦aig, var, frame, assign⟧sv where idx =/= (_ : Aig).addInput.snd
+
+@[simp, grind =] theorem denoteCV_input_getVar {idx : InputIdx} (valid : idx.validIn aig) : ⟦idx.getVar aig valid⟧cv = assign idx frame := by grind [denoteCV_get_input]
+@[simp, grind =] theorem denoteSV_input_getVar {idx : InputIdx} (valid : idx.validIn aig) : ⟦idx.getVar aig valid⟧sv = assign idx frame := by grind [denoteSV_get_input]
 
 @[simp]
-theorem denoteCombVar_mono {old new : Aig} {oldWf : old.WellFormed} {newWf : new.WellFormed}
-    (mono : old ≤ new) {var : Var} (valid : var.validIn old) :
-    new.denoteCombVar var assign newWf = old.denoteCombVar var assign oldWf := by
-  induction _ : var using WellFounded.induction generalizing var
+theorem denoteCV_get_latch_zero {idx : LatchIdx} (h : aig.get var valid = .latch idx) :
+    ⟦var⟧cv0 = assign idx 0 := by
+  grind [denoteCV_eq, denoteC]
+
+grind_pattern denoteCV_get_latch_zero => aig.get var, Node.latch idx, ⟦aig, var, 0, assign⟧cv where
+  idx =/= ((_ : Aig).addLatch _ _).snd
+
+@[simp]
+theorem denoteSV_get_latch_zero {idx : LatchIdx} (h : aig.get var valid = .latch idx) :
+    ⟦var⟧sv0 =
+    match idx.getReset aig with
+    | none       => assign idx 0
+    | some reset => ⟦reset⟧s0 := by
+  grind [denoteSV_eq, denoteS]
+
+grind_pattern denoteSV_get_latch_zero => aig.get var, Node.latch idx, ⟦aig, var, 0, assign⟧sv where
+  idx =/= ((_ : Aig).addLatch _ _).snd
+
+@[simp]
+theorem denoteCV_get_latch {idx : LatchIdx} (h : aig.get var valid = .latch idx) :
+    ⟦var⟧cv =
+    match frame with
+    | 0     => assign idx 0
+    | n + 1 => ⟦idx.getNext aig, n⟧c := by
+  grind [denoteCV, denoteC]
+
+grind_pattern denoteCV_get_latch => aig.get var, Node.latch idx, ⟦aig, var, frame, assign⟧cv where
+  idx =/= ((_ : Aig).addLatch _ _).snd
+  frame =/= 0
+
+@[simp]
+theorem denoteSV_get_latch {idx : LatchIdx} (h : aig.get var valid = .latch idx) :
+    ⟦var⟧sv =
+    match frame with
+    | 0            =>
+      match idx.getReset aig with
+      | none       => assign idx 0
+      | some reset => ⟦reset⟧s0
+    | n + 1        => ⟦idx.getNext aig, n⟧s := by
+  grind [denoteSV, denoteS]
+
+grind_pattern denoteSV_get_latch => aig.get var, Node.latch idx, ⟦aig, var, frame, assign⟧sv where
+  idx =/= ((_ : Aig).addLatch _ _).snd
+  frame =/= 0
+
+@[simp, grind =]
+theorem denoteCV_latch_getVar_zero {idx : LatchIdx} (valid : idx.validIn aig) :
+    ⟦idx.getVar aig valid⟧cv0 = assign idx 0 := by
+  grind [get_latch_getVar]
+
+@[simp, grind =]
+theorem denoteSV_latch_getVar_zero {idx : LatchIdx} (valid : idx.validIn aig) :
+    ⟦idx.getVar aig valid⟧sv0 =
+    match idx.getReset aig with
+    | none       => assign idx 0
+    | some reset => ⟦reset⟧s0 := by
+  grind [get_latch_getVar]
+
+@[simp]
+theorem denoteCV_latch_getVar {idx : LatchIdx} (valid : idx.validIn aig) :
+    ⟦idx.getVar aig valid⟧cv =
+    match frame with
+    | 0     => assign idx 0
+    | n + 1 => ⟦idx.getNext aig, n⟧c := by
+  grind [get_latch_getVar, denoteCV_get_latch]
+
+grind_pattern denoteCV_latch_getVar => ⟦aig, idx.getVar aig, frame, assign⟧cv where
+  frame =/= 0
+
+@[simp]
+theorem denoteSV_latch_getVar {idx : LatchIdx} (valid : idx.validIn aig) :
+    ⟦idx.getVar aig valid⟧sv =
+    match frame with
+    | 0            =>
+      match idx.getReset aig with
+      | none       => assign idx 0
+      | some reset => ⟦reset⟧s0
+    | n + 1        => ⟦idx.getNext aig, n⟧s := by
+  grind [get_latch_getVar, denoteCV_get_latch]
+
+grind_pattern denoteSV_latch_getVar => ⟦aig, idx.getVar aig, frame, assign⟧sv where
+  frame =/= 0
+
+@[simp] theorem denoteCV_get_and {rhs0 rhs1 : Lit} (h : aig.get var valid = .and rhs0 rhs1) : ⟦var⟧cv = (⟦rhs0⟧c && ⟦rhs1⟧c) := by grind [denoteCV, denoteC]
+@[simp] theorem denoteSV_get_and {rhs0 rhs1 : Lit} (h : aig.get var valid = .and rhs0 rhs1) : ⟦var⟧sv = (⟦rhs0⟧s && ⟦rhs1⟧s) := by grind [denoteSV, denoteS]
+grind_pattern denoteCV_get_and => aig.get var, Node.and rhs0 rhs1, ⟦aig, var, frame, assign⟧cv
+grind_pattern denoteSV_get_and => aig.get var, Node.and rhs0 rhs1, ⟦aig, var, frame, assign⟧sv
+
+end get
+
+section mono
+variable {old new : Aig} {oldWf : old.WellFormed} {newWf : new.WellFormed} (mono : old ≤ new)
+include mono
+
+theorem denoteC_mono (valid : lit.validIn old) :
+    ⟦new, lit, frame, assign⟧c = ⟦old, lit, frame, assign⟧c := by
+  induction _ : (frame, lit.var) using WellFounded.induction generalizing lit frame
   exact WellFoundedRelation.wf
   next ih _ =>
-    simp [WellFoundedRelation.rel] at ih
-    unfold denoteCombVar
+    simp only [WellFoundedRelation.rel, Prod.lex_def, InvImage, sizeOf_nat] at ih
+    unfold denoteC
     grind
 
-grind_pattern denoteCombVar_mono => new.denoteCombVar var assign newWf, old ≤ new
+grind_pattern denoteC_mono => ⟦new, lit, frame, assign⟧c, old ≤ new
+
+theorem denoteS_mono (valid : lit.validIn old) :
+    ⟦new, lit, frame, assign⟧s = ⟦old, lit, frame, assign⟧s := by
+  induction _ : (frame, lit.var) using WellFounded.induction generalizing lit frame
+  exact WellFoundedRelation.wf
+  next ih _ =>
+    simp only [WellFoundedRelation.rel, Prod.lex_def, InvImage, sizeOf_nat] at ih
+    unfold denoteS
+    grind
+
+grind_pattern denoteS_mono => ⟦new, lit, frame, assign⟧s, old ≤ new
+
+theorem denoteCV_mono (valid : var.validIn old) : ⟦new, var, frame, assign⟧cv = ⟦old, var, frame, assign⟧cv := by grind [denoteC_mono, denoteCV_eq]
+theorem denoteSV_mono (valid : var.validIn old) : ⟦new, var, frame, assign⟧sv = ⟦old, var, frame, assign⟧sv := by grind [denoteS_mono, denoteSV_eq]
+grind_pattern denoteCV_mono => ⟦new, var, frame, assign⟧cv, old ≤ new
+grind_pattern denoteSV_mono => ⟦new, var, frame, assign⟧sv, old ≤ new
+
+end mono
 
 open Std.Sat AIG in
-private theorem denoteComb_eq_std_denote {assign : LeafIdx -> Bool} :
-    aig.denoteComb lit assign wf =
+private theorem denoteC_eq_std_denote :
+    ⟦lit⟧c0 =
     if valid : lit.validIn aig then
-      AIG.denote assign (Entrypoint.mk aig.aig <| lit.toRef valid)
+      AIG.denote (assign · 0) (Entrypoint.mk aig.aig <| lit.toRef valid)
     else
       lit.inverted := by
   induction h : lit.var using WellFounded.induction generalizing lit
@@ -150,361 +414,168 @@ private theorem denoteComb_eq_std_denote {assign : LeafIdx -> Bool} :
     split
     case isTrue valid =>
       cases h : aig[lit.var] with
-      | false => clear ih; grind [get_eq_getElem_decls_false]
-      | input idx => clear ih; grind [get_eq_getElem_decls_input]
-      | latch idx => clear ih; grind [get_eq_getElem_decls_latch]
+      | false     => clear ih; grind [get_eq_getElem_decls_false valid h]
+      | input idx => clear ih; grind [get_eq_getElem_decls_input valid h]
+      | latch idx => clear ih; grind [get_eq_getElem_decls_latch valid h]
       | and rhs0 rhs1 =>
-        rw [denoteComb_eq, denoteCombVar_get_and h, ih rhs0.var, ih rhs1.var]
+        rw [denoteC_eq, denoteCV_get_and h, ih rhs0.var, ih rhs1.var]
         · unfold AIG.denote
           grind [get_eq_getElem_decls_and valid h]
         all_goals (clear ih; grind)
     case isFalse => grind
 
-@[simp, grind =]
-theorem denoteCombVar_addInput'_self {idx : InputIdx} {wf : (aig.addInput' idx).WellFormed} :
-    (aig.addInput' idx).denoteCombVar (idx.getVar (aig.addInput' idx)) assign wf =
-    assign idx := by
-  grind
+section addInput'
+variable {idx : InputIdx} {wf : (aig.addInput' idx).WellFormed}
 
-@[simp, grind =]
-theorem denoteCombVar_addLatch'_self {idx : LatchIdx} {next : Lit} {reset : Option Lit}
-    (wf : (aig.addLatch' idx next reset).WellFormed) :
-    (aig.addLatch' idx next reset).denoteCombVar
-      (idx.getVar (aig.addLatch' idx next reset)) assign wf =
-    assign idx := by
-  grind
+@[simp, grind =] theorem denoteCV_addInput'_self : ⟦aig.addInput' idx, idx.getVar (aig.addInput' idx), frame, assign⟧cv = assign idx frame := by grind
+@[simp, grind =] theorem denoteSV_addInput'_self : ⟦aig.addInput' idx, idx.getVar (aig.addInput' idx), frame, assign⟧sv = assign idx frame := by grind
 
-@[simp, grind =]
-theorem denoteComb_addAnd_self {rhs0 rhs1 : Lit} (h0 : rhs0.validIn aig) (h1 : rhs1.validIn aig)
-    (wf' : (aig.addAnd rhs0 rhs1 h0 h1).fst.WellFormed) :
-    (aig.addAnd rhs0 rhs1 h0 h1).fst.denoteComb (aig.addAnd rhs0 rhs1 h0 h1).snd assign wf' =
-    (aig.denoteComb rhs0 assign wf && aig.denoteComb rhs1 assign wf) := by
-  have : (aig.addAnd rhs0 rhs1 h0 h1).snd.validIn (aig.addAnd rhs0 rhs1 h0 h1).fst := by grind
-  simp only [denoteComb_eq_std_denote, this]
-  simp only [addAnd, Lit.toRef_ofRef]
-  rw [Std.Sat.AIG.denote_mkAndCached]
-  grind [denoteComb_eq_std_denote]
+end addInput'
 
--- TODO: Prove that latch setters don't affect the comb denotation
-
-end denoteComb
-
-mutual
-
-/--
-Denotation of the sequential semantics of the Aig in each timeframe, taking a function to assign
-values to the inputs in each frame.
--/
-def denoteVar (aig : Aig) (var : Var) (frame : Frame) (assign : LeafIdx -> Frame -> Bool)
-      (wf : aig.WellFormed := by grind) : Bool :=
-    match _ : aig[var]? with
-    | none
-    | some .false           => false
-    | some (.input idx)     => assign idx frame
-    | some (.latch idx)     =>
-      match frame with
-      | 0                   =>
-        match _ : idx.getReset aig with
-        | none              => assign idx frame
-        | some reset        => aig.denote reset 0 assign
-      | n + 1               => aig.denote (idx.getNext aig) n assign
-    | some (.and rhs0 rhs1) => aig.denote rhs0 frame assign && aig.denote rhs1 frame assign
-  termination_by (frame, var, 0)
-  decreasing_by all_goals grind
-
-def denote (aig : Aig) (lit : Lit) (frame : Frame) (assign : LeafIdx -> Frame -> Bool)
-    (wf : aig.WellFormed := by grind) : Bool :=
-  lit.inverted ^^ aig.denoteVar lit.var frame assign
-  termination_by (frame, lit.var, 1)
-
-end -- mutual
-
-def denoteResetVar (aig : Aig) (var : Var) (assign : LeafIdx -> Bool) (wf : aig.WellFormed := by grind) : Bool :=
-  aig.denoteVar var 0 (fun idx _ => assign idx) wf
-
-@[simp, grind =]
-theorem denoteResetVar_eq {var : Var} {assign wf} :
-    aig.denoteResetVar var assign wf = aig.denoteVar var 0 (fun idx _ => assign idx) wf := by
-  rfl
-
-def denoteReset (aig : Aig) (lit : Lit) (assign : LeafIdx -> Bool) (wf : aig.WellFormed := by grind) : Bool :=
-  aig.denote lit 0 (fun idx _ => assign idx) wf
-
-@[simp, grind =]
-theorem denoteReset_eq {lit : Lit} {assign wf} :
-    aig.denoteReset lit assign wf = aig.denote lit 0 (fun idx _ => assign idx) wf := by
-  rfl
-
-theorem denoteReset_eq_denoteResetVar {lit : Lit} {assign wf} :
-    aig.denoteReset lit assign wf = (lit.inverted ^^ aig.denoteResetVar lit.var assign wf) := by
-  simp [denote]
-
-
-/--
-To allow reasoning about different possible interpretations of the leaves of the Aig (e.g. when
-constructing latches where the next state function hasn't been built yet), we design the semantics
-around an arbitrary semantics for the leaves.
-
-This function defines the concrete semantics that are used in practice in `denote`/`denoteVar` for
-defining sequential computation, allowing an external semantics to be shown equivalent by showing
-equivalence to this.
--/
-@[expose]
-def assignSeq (aig : Aig) (frame : Frame) (assign : LeafIdx -> Frame -> Bool) (wf : aig.WellFormed := by grind) :
-    LeafIdx -> Bool :=
-  fun idx =>
-    match _ : idx with
-    | .input idx => assign idx frame
-    | .latch idx =>
-      if h : idx.validIn aig then
-        match frame with
-        | 0 =>
-          match idx.getReset aig with
-          | none       => assign idx 0
-          | some reset => aig.denote reset 0 assign
-        | n + 1        => aig.denote (idx.getNext aig)  n assign
-      else
-        false
-
-section denote
-variable {assign : LeafIdx -> Frame -> Bool}
-
-@[simp, grind =]
-theorem assignSeq_input (idx : InputIdx) :
-    (aig.assignSeq frame assign wf) idx = assign idx frame := by
-  simp [assignSeq]
-
-@[simp, grind =]
-theorem assignSeq_latch {idx : LatchIdx} (valid : idx.validIn aig) :
-    (aig.assignSeq frame assign wf) idx =
-    match frame with
-    | 0 =>
-      match idx.getReset aig with
-      | none       => assign idx 0
-      | some reset => aig.denote reset 0 assign
-    | n + 1        => aig.denote (idx.getNext aig) n assign := by
-  simp [assignSeq, valid]
-
-@[simp, grind =]
-theorem assignSeq_latch_invalid {idx : LatchIdx} (invalid : ¬idx.validIn aig) :
-    (aig.assignSeq frame assign wf) idx = false := by
-  simp [assignSeq, invalid]
-
-@[simp, grind =]
-theorem denote_eq :
-    aig.denote lit frame assign wf =
-    (lit.inverted ^^ aig.denoteVar lit.var frame assign wf) := by
-  rw [denote]
-
-@[local grind =]
-theorem denoteVar_eq_denoteCombVar :
-    aig.denoteVar var frame assign wf =
-    aig.denoteCombVar var (aig.assignSeq frame assign wf) wf := by
-  induction h : (frame, var) using WellFounded.induction generalizing var frame
-  exact WellFoundedRelation.wf
-  next ih =>
-    simp [WellFoundedRelation.rel, Prod.lex_def, InvImage] at ih
-    rw [denoteVar, denoteCombVar]
-    grind
-
-theorem denote_eq_denoteComb :
-    aig.denote lit frame assign wf =
-    aig.denoteComb lit (aig.assignSeq frame assign wf) wf := by
-  simp only [denote_eq, denoteVar_eq_denoteCombVar, denoteComb_eq]
-
--- TODO: Rebuild all the basic denotations on denoteVar, the same as denoteCombVar
-
-@[simp, grind =]
-theorem denoteVar_constant :
-    aig.denoteVar .constant frame assign wf = false := by
-  grind
-
-@[simp]
-theorem denoteVar_invalid (invalid : ¬var.validIn aig) :
-    aig.denoteVar var frame assign wf = false := by
-  grind
-
-grind_pattern denoteVar_invalid => aig.denoteVar var frame assign wf, var.validIn aig
-
-@[simp]
-theorem denoteVar_get_false (h : aig.get var valid = .false) :
-    aig.denoteVar var frame assign wf = false := by
-  grind
-
-grind_pattern denoteVar_get_false => aig.get var, Node.false, aig.denoteVar var frame assign wf
-
-@[simp]
-theorem denoteVar_get_input {idx : InputIdx} (h : aig.get var valid = .input idx) :
-    aig.denoteVar var frame assign wf = assign idx frame := by
-  grind
-
-grind_pattern denoteVar_get_input => aig.get var, Node.input idx, aig.denoteVar var frame assign wf where
-  var =/= idx.getVar aig
-  idx =/= (_ : Aig).addInput.snd
-
-@[simp, grind =]
-theorem denoteVar_input_getVar {idx : InputIdx} (valid : idx.validIn aig) :
-    aig.denoteVar (idx.getVar aig valid) frame assign wf = assign idx frame := by
-  grind
-
-@[simp]
-theorem denoteVar_get_latch {idx : LatchIdx} (h : aig.get var valid = .latch idx) :
-    aig.denoteVar var frame assign wf =
-    match frame with
-    | 0 =>
-      match idx.getReset aig with
-      | none       => assign idx 0
-      | some reset => aig.denote reset 0 assign wf
-    | n + 1 => aig.denote (idx.getNext aig) n assign wf := by
-  grind
-
-grind_pattern denoteVar_get_latch => aig.get var, Node.latch idx, aig.denoteVar var frame assign wf where
-  var =/= idx.getVar aig
-  idx =/= ((_ : Aig).addLatch' _ _ _)
-
-@[simp, grind =]
-theorem denoteVar_latch_getVar {idx : LatchIdx} (valid : idx.validIn aig) :
-    aig.denoteVar (idx.getVar aig valid) frame assign wf =
-    match frame with
-    | 0 =>
-      match idx.getReset aig with
-      | none       => assign idx 0
-      | some reset => aig.denote reset 0 assign wf
-    | n + 1 => aig.denote (idx.getNext aig) n assign wf := by
-  grind
-
-@[simp]
-theorem denoteVar_get_and {rhs0 rhs1 : Lit} (h : aig.get var valid = .and rhs0 rhs1) :
-    aig.denoteVar var frame assign wf =
-      (aig.denote rhs0 frame assign wf && aig.denote rhs1 frame assign wf) := by
-  grind
-
-grind_pattern denoteVar_get_and => aig.get var, Node.and rhs0 rhs1, aig.denoteVar var frame assign wf
-
-theorem denoteVar_eq_of_le (assign assign' : LeafIdx -> Frame -> Bool)
-    (h : {idx : LeafIdx} -> (valid : idx.validIn aig) -> {frame' : Frame} ->
-      frame' < frame ∨ (frame' = frame ∧ idx.getVar aig valid ≤ var) ->
-      assign' idx frame' = assign idx frame') :
-    aig.denoteVar var frame assign' wf = aig.denoteVar var frame assign wf := by
-  induction h : (frame, var) using WellFounded.induction generalizing frame var
-  exact WellFoundedRelation.wf
-  next ih _ =>
-    simp only [WellFoundedRelation.rel, Prod.lex_def, InvImage, sizeOf_nat] at ih
-    simp only [denoteVar_eq_denoteCombVar]
-    apply denoteCombVar_eq_of_le
-    case h =>
-      unfold assignSeq
-      cases frame
-      · grind (splits := 15)
-      · grind
-    all_goals trivial
-
-section mono
-variable {old new : Aig} {oldWf : old.WellFormed} {newWf : new.WellFormed} (mono : old ≤ new)
-include mono
-
-@[simp]
-theorem assignSeq_mono {idx : LeafIdx} (valid : idx.validIn old) :
-    (new.assignSeq frame assign newWf) idx = (old.assignSeq frame assign oldWf) idx := by
-  induction h : (frame, idx.getVar old valid) using WellFounded.induction generalizing frame idx
-  exact WellFoundedRelation.wf
-  next ih =>
-    simp only [WellFoundedRelation.rel, Prod.lex_def, InvImage, sizeOf_nat] at ih
-    unfold assignSeq
-    cases idx with
-    | input _ => clear ih; grind only
-    | latch idx =>
-      cases h : idx.getReset old with
-      | none =>
-        cases frame <;> grind [denoteCombVar_eq_of_le]
-      | some reset =>
-        have : reset.var < idx.getVar old := by clear ih; grind
-        cases frame <;> grind [denoteCombVar_eq_of_le]
-
-grind_pattern assignSeq_mono => (new.assignSeq frame assign newWf) idx, old ≤ new
-
-@[simp]
-theorem denoteVar_mono (var : Var) (valid : var.validIn old) :
-    new.denoteVar var frame assign newWf = old.denoteVar var frame assign oldWf := by
-  grind [denoteCombVar_mono mono, denoteCombVar_eq_of_le]
-
-grind_pattern denoteVar_mono => new.denoteVar var frame assign newWf, old ≤ new
-
-end mono
-
-@[simp, grind =]
-theorem denoteVar_addInput'_self {idx : InputIdx} (wf : (aig.addInput' idx).WellFormed) :
-    (aig.addInput' idx).denoteVar (idx.getVar (aig.addInput' idx)) frame assign wf =
-    assign idx frame := by
-  grind
-
-section addLatch'
+section addLatch
 variable {idx : LatchIdx} {next : Lit} {reset : Option Lit}
+variable (wf : (aig.addLatch' idx next reset).WellFormed)
 
-@[simp]
-theorem denoteVar_addLatch'_self_none (nextValid : next.validIn aig) (h : ¬idx.validIn aig) :
-    let res := aig.addLatch' idx next none
-    res.denoteVar (idx.getVar res) frame assign =
-    match frame with
-    | 0 => assign idx 0
-    | n + 1 => aig.denote next n assign wf := by
+@[simp, grind =]
+theorem denoteCV_addLatch'_self_zero :
+    ⟦aig.addLatch' idx next reset, idx.getVar (aig.addLatch' idx next reset), assign⟧cv0 =
+    assign idx 0 := by
   grind
 
 @[simp]
-theorem denoteVar_addLatch'_self_some {reset : Lit} (nextValid : next.validIn aig)
-    (resetValid : reset.validIn aig) (h : ¬idx.validIn aig) :
-    let res := aig.addLatch' idx next <| some reset
-    res.denoteVar (idx.getVar res) frame assign =
-    match frame with
-    | 0 => aig.denote reset 0 assign wf
-    | n + 1 => aig.denote next n assign wf := by
+theorem denoteSV_addLatch'_self_zero_none (wf : (aig.addLatch' idx next none).WellFormed) :
+    ⟦aig.addLatch' idx next none, idx.getVar (aig.addLatch' idx next none), assign⟧sv0 =
+    assign idx 0 := by
   grind
 
-theorem denoteVar_addLatch'_self (nextValid : next.validIn aig)
+@[simp]
+theorem denoteSV_addLatch'_self_zero_some {reset : Lit}
+    (wf : (aig.addLatch' idx next <| some reset).WellFormed)
+    (resetValid : reset.validIn aig)
+    (h : ¬idx.validIn aig) :
+    ⟦aig.addLatch' idx next <| some reset, idx.getVar (aig.addLatch' idx next <| some reset), assign⟧sv0 =
+    ⟦reset⟧s0 := by
+  grind
+
+@[simp, grind =]
+theorem denoteSV_addLatch'_self_zero
+    (wf : (aig.addLatch' idx next reset).WellFormed)
     (resetValid :
       match reset with
       | none => True
-      | some lit => lit.validIn aig)
+      | some reset => reset.validIn aig)
     (h : ¬idx.validIn aig) :
-    let res := aig.addLatch' idx next reset
-    res.denoteVar (idx.getVar res) frame assign =
-    match frame with
-    | 0 =>
-      match reset with
-      | none => assign idx 0
-      | some lit => aig.denote lit 0 assign wf
-    | n + 1 => aig.denote next n assign wf := by
-  grind [denoteVar_addLatch'_self_none, denoteVar_addLatch'_self_some]
-
-grind_pattern denoteVar_addLatch'_self =>
-  (aig.addLatch' idx next reset).denoteVar (idx.getVar (aig.addLatch' idx next reset)) frame assign
-
-end addLatch'
+    ⟦aig.addLatch' idx next reset, idx.getVar (aig.addLatch' idx next reset), assign⟧sv0 =
+    match reset with
+    | none       => assign idx 0
+    | some reset => ⟦reset⟧s0 := by
+  grind
 
 @[simp, grind =]
-theorem denote_addAnd_self {rhs0 rhs1 : Lit} (h0 : rhs0.validIn aig) (h1 : rhs1.validIn aig)
-    (wf' : (aig.addAnd rhs0 rhs1 h0 h1).fst.WellFormed) :
-    (aig.addAnd rhs0 rhs1 h0 h1).fst.denote (aig.addAnd rhs0 rhs1 h0 h1).snd frame assign wf' =
-    (aig.denote rhs0 frame assign wf && aig.denote rhs1 frame assign wf) := by
-  grind [denote_eq_denoteComb, denoteCombVar_mono, denoteCombVar_eq_of_le]
+theorem denoteCV_addLatch'_self {idx : LatchIdx} {next : Lit} {reset : Option Lit}
+    (wf : (aig.addLatch' idx next reset).WellFormed)
+    (nextValid : next.validIn aig)
+    (h : ¬idx.validIn aig) :
+    ⟦aig.addLatch' idx next reset, idx.getVar (aig.addLatch' idx next reset), frame, assign⟧cv =
+    match frame with
+    | 0     => assign idx 0
+    | n + 1 => ⟦next, n⟧c := by
+  grind
 
-end denote
+grind_pattern denoteCV_addLatch'_self => ⟦aig.addLatch' idx next reset, idx.getVar (aig.addLatch' idx next reset), frame, assign⟧cv where
+  frame =/= 0
+
+@[simp, grind =]
+theorem denoteSV_addLatch'_self
+    (wf : (aig.addLatch' idx next reset).WellFormed)
+    (resetValid :
+      match reset with
+      | none => True
+      | some reset => reset.validIn aig)
+    (nextValid : next.validIn aig)
+    (h : ¬idx.validIn aig) :
+    ⟦aig.addLatch' idx next reset, idx.getVar (aig.addLatch' idx next reset), frame, assign⟧sv =
+    match frame with
+    | 0            =>
+      match reset with
+      | none       => assign idx 0
+      | some reset => ⟦reset⟧s0
+    | n + 1        => ⟦next, n⟧s := by
+  grind
+
+grind_pattern denoteSV_addLatch'_self => ⟦aig.addLatch' idx next reset, idx.getVar (aig.addLatch' idx next reset), frame, assign⟧sv where
+  frame =/= 0
+
+end addLatch
+
+section addAnd
+variable {rhs0 rhs1 : Lit} (h0 : rhs0.validIn aig) (h1 : rhs1.validIn aig)
+
+@[simp]
+theorem denoteC_addAnd_self :
+    let res := aig.addAnd rhs0 rhs1 h0 h1
+    ⟦res.fst, res.snd, frame, assign⟧c = (⟦rhs0⟧c && ⟦rhs1⟧c) := by
+  intro res
+  suffices h : ∀ (assign), ⟦res.fst, res.snd, assign⟧c0 = (⟦aig, rhs0, assign⟧c0 && ⟦aig, rhs1, assign⟧c0) by
+    have : denoteC.assignNext res.fst frame assign = denoteC.assignNext aig frame assign := by
+      funext _ _
+      unfold denoteC.assignNext
+      grind
+    conv =>
+      pattern (occs := *) ⟦_, _, frame, _⟧c
+      <;> rw [denoteC_eq_denoteC_assignNext]
+    simp only [this, h]
+  intro assign
+  simp only [res, denoteC_eq_std_denote]
+  split
+  · simp only [addAnd, Lit.toRef_ofRef]
+    rw [Std.Sat.AIG.denote_mkAndCached]
+  · grind
+
+grind_pattern denoteC_addAnd_self => ⟦(aig.addAnd rhs0 rhs1 h0 h1).fst, (aig.addAnd rhs0 rhs1 h0 h1).snd, frame, assign⟧c
+
+@[simp]
+theorem denoteS_addAnd_self :
+    let res := aig.addAnd rhs0 rhs1 h0 h1
+    ⟦res.fst, res.snd, frame, assign⟧s = (⟦rhs0⟧s && ⟦rhs1⟧s) := by
+  intro res
+  have : denoteS.assignNext res.fst frame assign = denoteS.assignNext aig frame assign := by
+    funext _ _
+    unfold denoteS.assignNext
+    grind
+  simp only [denoteS_eq_denoteC_assignNext]
+  grind
+
+grind_pattern denoteS_addAnd_self => ⟦(aig.addAnd rhs0 rhs1 h0 h1).fst, (aig.addAnd rhs0 rhs1 h0 h1).snd, frame, assign⟧s
+
+end addAnd
 
 /--
 A literal is unsatisfiable in an Aig if for all assignments to inputs and latches its value is
 false.
 -/
-@[expose]
-def Unsat (aig : Aig) (lit : Lit) (wf : aig.WellFormed := by grind) :=
+def Unsat (aig : Aig) (lit : Lit) (wf : aig.WellFormed := by grind) : Prop :=
   ∀ {assign},
-    aig.denoteComb lit assign wf = false
+    ⟦aig, lit, assign⟧c0 = false
+
+theorem Unsat_iff :
+    aig.Unsat lit ↔
+    (∀ (assign : LeafIdx -> Bool), ⟦aig, lit, fun idx _ => assign idx⟧c0 = false) := by
+  unfold Unsat
+  constructor
+  · grind
+  · intro h assign
+    rw [denoteC_zero_eq_assign_zero]
+    grind [h (fun idx => assign idx 0)]
 
 open Std.Sat AIG in
-private theorem Unsat_iff_std_Unsat :
+private theorem Unsat_iff_std_Unsat (valid : lit.validIn aig) :
     aig.Unsat lit wf ↔
-    Entrypoint.Unsat (.mk aig.aig <| lit.toRef litValid) := by
-  simp only [Unsat, AIG.Entrypoint.Unsat, AIG.UnsatAt, denoteComb_eq_std_denote, litValid]
-  grind only
+    Entrypoint.Unsat (.mk aig.aig <| lit.toRef valid) := by
+  rw [Unsat_iff]
+  · simp only [AIG.Entrypoint.Unsat, AIG.UnsatAt, denoteC_eq_std_denote, valid]
+    grind
+  · grind
 
 /--
 A literal is unreachable if there is no trace that can reach a state where it is true.
@@ -512,11 +583,4 @@ A literal is unreachable if there is no trace that can reach a state where it is
 @[expose]
 def Unreachable (aig : Aig) (lit : Lit) (wf : aig.WellFormed := by grind) :=
   ∀ {frame assign},
-    aig.denote lit frame assign wf = false
-
-theorem Unreachable_of_induction
-    (init : ∀ {assign}, aig.denote lit 0 assign wf = false)
-    (trans : ∀ {frame assign}, aig.denote lit frame assign wf = false → aig.denote lit (frame + 1) assign wf = false) :
-    aig.Unreachable lit wf := by
-  intro frame
-  induction h : frame generalizing frame <;> grind
+    ⟦aig, lit, frame, assign⟧s = false
